books/models/jvm/m5/demo.lisp
@@ -104,33 +104,33 @@ Below is the output of jvm2acl2 for M5.
      "Demo"
      '("java.lang.Object")
      '()
-     '("ans")
+     '("ans:I")
      '()
      (list
-      '("<init>()V" () nil
+      '("<init>:()V" () nil
         (aload_0)
-        (invokespecial "java.lang.Object" "<init>()V" 0)
+        (invokespecial "java.lang.Object" "<init>:()V" 0)
         (return))
-      '("fact(I)I" (int) nil
+      '("fact:(I)I" (int) nil
         (iload_0)
         (ifle LABEL::TAG_0)
         (iload_0)
         (iload_0)
         (iconst_1)
         (isub)
-        (invokestatic "Demo" "fact(I)I" 1)
+        (invokestatic "Demo" "fact:(I)I" 1)
         (imul)
         (ireturn)
         (LABEL::TAG_0 iconst_1)
         (ireturn))
-      '("main([Ljava/lang/String;)V" (java.lang.String[]) nil
+      '("main:([Ljava/lang/String;)V" (java.lang.String[]) nil
         (iconst_4)
         (istore_1)
         (iload_1)
         (iconst_1)
         (iadd)
-        (invokestatic "Demo" "fact(I)I" 1)
-        (putstatic "Demo" "ans" nil)
+        (invokestatic "Demo" "fact:(I)I" 1)
+        (putstatic "Demo" "ans:I")
         (return)))
      '(REF -1)))))
 
@@ -140,8 +140,8 @@ Below is the output of jvm2acl2 for M5.
     (iload_1)
     (iconst_1)
     (iadd)
-    (invokestatic "Demo" "fact(I)I" 1)
-    (putstatic "Demo" "ans" nil)
+    (invokestatic "Demo" "fact:(I)I" 1)
+    (putstatic "Demo" "ans:I")
     (return)))
 
 (defun Demo-ms ()
@@ -167,8 +167,8 @@ Below is the output of jvm2acl2 for M5.
           (ILOAD_1)
           (ICONST_1)
           (IADD)
-          (INVOKESTATIC "Demo" "fact(I)I" 1)
-          (PUTSTATIC "Demo" "ans" NIL)
+          (INVOKESTATIC "Demo" "fact:(I)I" 1)
+          (PUTSTATIC "Demo" "ans:I")
           (RETURN))
          UNLOCKED "Demo"))
      SCHEDULED NIL))
@@ -193,12 +193,12 @@ Below is the output of jvm2acl2 for M5.
       ("mcount" . 0)
       ("wait-set" . 0)))
   (5 ("java.lang.Class" ("<name>" . "Demo")
-      ("ans" . 0))
+      ("ans:I" . 0))
      ("java.lang.Object" ("monitor" . 0)
       ("mcount" . 0)
       ("wait-set" . 0))))
  (("java.lang.Object" NIL ("monitor" "mcount" "wait-set")
-   NIL NIL (("<init>()V" NIL NIL (RETURN)))
+   NIL NIL (("<init>:()V" NIL NIL (RETURN)))
    (REF 0))
   ("ARRAY" ("java.lang.Object")
    (("<array>" . *ARRAY*))
@@ -206,53 +206,53 @@ Below is the output of jvm2acl2 for M5.
   ("java.lang.Thread"
    ("java.lang.Object")
    NIL NIL NIL
-   (("run()V" NIL NIL (RETURN))
-    ("start()V" NIL NIL NIL)
-    ("stop()V" NIL NIL NIL)
-    ("<init>()V" NIL NIL (ALOAD_0)
-     (INVOKESPECIAL "java.lang.Object" "<init>()V" 0)
+   (("run:()V" NIL NIL (RETURN))
+    ("start:()V" NIL NIL NIL)
+    ("stop:()V" NIL NIL NIL)
+    ("<init>:()V" NIL NIL (ALOAD_0)
+     (INVOKESPECIAL "java.lang.Object" "<init>:()V" 0)
      (RETURN)))
    (REF 2))
   ("java.lang.String"
    ("java.lang.Object")
    ("strcontents")
    NIL NIL
-   (("<init>()V" NIL NIL (ALOAD_0)
-     (INVOKESPECIAL "java.lang.Object" "<init>()V" 0)
+   (("<init>:()V" NIL NIL (ALOAD_0)
+     (INVOKESPECIAL "java.lang.Object" "<init>:()V" 0)
      (RETURN)))
    (REF 3))
   ("java.lang.Class" ("java.lang.Object")
    NIL NIL NIL
-   (("<init>()V" NIL NIL (ALOAD_0)
-     (INVOKESPECIAL "java.lang.Object" "<init>()V" 0)
+   (("<init>:()V" NIL NIL (ALOAD_0)
+     (INVOKESPECIAL "java.lang.Object" "<init>:()V" 0)
      (RETURN)))
    (REF 4))
   ("Demo" ("java.lang.Object")
-   NIL ("ans")
+   NIL ("ans:I")
    NIL
-   (("<init>()V" NIL NIL (ALOAD_0)
-     (INVOKESPECIAL "java.lang.Object" "<init>()V" 0)
+   (("<init>:()V" NIL NIL (ALOAD_0)
+     (INVOKESPECIAL "java.lang.Object" "<init>:()V" 0)
      (RETURN))
-    ("fact(I)I" (INT)
+    ("fact:(I)I" (INT)
      NIL (ILOAD_0)
      (IFLE 12)
      (ILOAD_0)
      (ILOAD_0)
      (ICONST_1)
      (ISUB)
-     (INVOKESTATIC "Demo" "fact(I)I" 1)
+     (INVOKESTATIC "Demo" "fact:(I)I" 1)
      (IMUL)
      (IRETURN)
      (ICONST_1)
      (IRETURN))
-    ("main([Ljava/lang/String;)V" (|JAVA.LANG.STRING[]|)
+    ("main:([Ljava/lang/String;)V" (|JAVA.LANG.STRING[]|)
      NIL (ICONST_4)
      (ISTORE_1)
      (ILOAD_1)
      (ICONST_1)
      (IADD)
-     (INVOKESTATIC "Demo" "fact(I)I" 1)
-     (PUTSTATIC "Demo" "ans" NIL)
+     (INVOKESTATIC "Demo" "fact:(I)I" 1)
+     (PUTSTATIC "Demo" "ans:I")
      (RETURN)))
    (REF 5))))
 |#
@@ -276,8 +276,8 @@ Below is the output of jvm2acl2 for M5.
                (ILOAD\_1)
                (ICONST\_1)
                (IADD)
-               (INVOKESTATIC "Demo" "fact(I)I" 1)
-               (PUTSTATIC "Demo" "ans" NIL)
+               (INVOKESTATIC "Demo" "fact:(I)I" 1)
+               (PUTSTATIC "Demo" "ans:I")
                (RETURN))
              'UNLOCKED
              "Demo")
@@ -318,7 +318,7 @@ Below is the output of jvm2acl2 for M5.
            ("wait-set" . 0))))
     (5 . (("java.lang.Class"
            ("<name>" . "Demo")
-           ("ans" . 0))
+           ("ans:I" . 0))
           ("java.lang.Object"
            ("monitor" . 0)
            ("mcount" . 0)
@@ -330,7 +330,7 @@ Below is the output of jvm2acl2 for M5.
      ("monitor" "mcount" "wait-set")
      NIL
      NIL
-     (("<init>()V" NIL NIL (RETURN)))
+     (("<init>:()V" NIL NIL (RETURN)))
      (REF 0))
     ("ARRAY"
      ("java.lang.Object")
@@ -344,11 +344,11 @@ Below is the output of jvm2acl2 for M5.
      NIL
      NIL
      NIL
-     (("run()V" NIL NIL (RETURN))
-      ("start()V" NIL NIL NIL)
-      ("stop()V" NIL NIL NIL)
-      ("<init>()V" NIL NIL (ALOAD\_0)
-       (INVOKESPECIAL "java.lang.Object" "<init>()V" 0)
+     (("run:()V" NIL NIL (RETURN))
+      ("start:()V" NIL NIL NIL)
+      ("stop:()V" NIL NIL NIL)
+      ("<init>:()V" NIL NIL (ALOAD\_0)
+       (INVOKESPECIAL "java.lang.Object" "<init>:()V" 0)
        (RETURN)))
      (REF 2))
     ("java.lang.String"
@@ -356,9 +356,9 @@ Below is the output of jvm2acl2 for M5.
      ("strcontents")
      NIL
      NIL
-     (("<init>()V" NIL NIL
+     (("<init>:()V" NIL NIL
        (ALOAD\_0)
-       (INVOKESPECIAL "java.lang.Object" "<init>()V" 0)
+       (INVOKESPECIAL "java.lang.Object" "<init>:()V" 0)
        (RETURN)))
      (REF 3))
     ("java.lang.Class"
@@ -366,40 +366,40 @@ Below is the output of jvm2acl2 for M5.
      NIL
      NIL
      NIL
-     (("<init>()V" NIL NIL
+     (("<init>:()V" NIL NIL
        (ALOAD\_0)
-       (INVOKESPECIAL "java.lang.Object" "<init>()V" 0)
+       (INVOKESPECIAL "java.lang.Object" "<init>:()V" 0)
        (RETURN)))
      (REF 4))
     ("Demo"
      ("java.lang.Object")
      NIL
-     ("ans")
+     ("ans:I")
      NIL
-     (("<init>()V" NIL NIL
+     (("<init>:()V" NIL NIL
        (ALOAD\_0)
-       (INVOKESPECIAL "java.lang.Object" "<init>()V" 0)
+       (INVOKESPECIAL "java.lang.Object" "<init>:()V" 0)
        (RETURN))
-      ("fact(I)I" (INT) NIL
+      ("fact:(I)I" (INT) NIL
        (ILOAD\_0)
        (IFLE 12)
        (ILOAD\_0)
        (ILOAD\_0)
        (ICONST\_1)
        (ISUB)
-       (INVOKESTATIC "Demo" "fact(I)I" 1)
+       (INVOKESTATIC "Demo" "fact:(I)I" 1)
        (IMUL)
        (IRETURN)
        (ICONST\_1)
        (IRETURN))
-      ("main([Ljava/lang/String;)V" (|JAVA.LANG.STRING[]|) NIL
+      ("main:([Ljava/lang/String;)V" (|JAVA.LANG.STRING[]|) NIL
        (ICONST\_4)
        (ISTORE\_1)
        (ILOAD\_1)
        (ICONST\_1)
        (IADD)
-       (INVOKESTATIC "Demo" "fact(I)I" 1)
-       (PUTSTATIC "Demo" "ans" NIL)
+       (INVOKESTATIC "Demo" "fact:(I)I" 1)
+       (PUTSTATIC "Demo" "ans:I")
        (RETURN)))
      (REF 5))))
 
@@ -454,7 +454,7 @@ Below is the output of jvm2acl2 for M5.
           (repeat th 2)))
 
 (defthm sample-execution
-  (equal (static-field-value "Demo" "ans"
+  (equal (static-field-value "Demo" "ans:I"
                              (run (main-sched 0) *Demo-state*))
          120)
   :rule-classes nil)
@@ -476,7 +476,7 @@ Below is the output of jvm2acl2 for M5.
      (format t "Schedule length:  ~a.~%" (len sched))
      (time
       (static-field-value
-       "Demo" "ans"
+       "Demo" "ans:I"
        (run sched
             (make-state
              (list
@@ -488,8 +488,8 @@ Below is the output of jvm2acl2 for M5.
                        (list n)
                        nil
                        '((ILOAD\_0)
-                         (INVOKESTATIC "Demo" "fact(I)I" 1)
-                         (PUTSTATIC "Demo" "ans" NIL)
+                         (INVOKESTATIC "Demo" "fact:(I)I" 1)
+                         (PUTSTATIC "Demo" "ans:I")
                          (RETURN))
                        'UNLOCKED
                        "Demo")
@@ -512,14 +512,14 @@ T
 ; Proving Fact Correct
 
 (defconst *fact-def*
-  '("fact(I)I" (INT) NIL
+  '("fact:(I)I" (INT) NIL
     (ILOAD_0)                         ;;;  0
     (IFLE 12)                         ;;;  1
     (ILOAD_0)                         ;;;  4
     (ILOAD_0)                         ;;;  5
     (ICONST_1)                        ;;;  6
     (ISUB)                            ;;;  7
-    (INVOKESTATIC "Demo" "fact(I)I" 1)    ;;;  8
+    (INVOKESTATIC "Demo" "fact:(I)I" 1)    ;;;  8
     (IMUL)                            ;;; 11
     (IRETURN)                         ;;; 12
     (ICONST_1)                        ;;; 13
@@ -527,10 +527,10 @@ T
 
 (defun poised-to-invoke-fact (th s n)
   (and (equal (status th s) 'SCHEDULED)
-       (equal (next-inst th s) '(invokestatic "Demo" "fact(I)I" 1))
+       (equal (next-inst th s) '(invokestatic "Demo" "fact:(I)I" 1))
        (equal n (top (stack (top-frame th s))))
        (intp n)
-       (equal (lookup-class-method "fact(I)I" "Demo" (class-table s))
+       (equal (lookup-class-method "fact:(I)I" "Demo" (class-table s))
               (cons "Demo" *fact-def*))))
 
 (defun induction-hint (th s n)
@@ -649,7 +649,7 @@ T
                                  (iload_3)
                                  (iconst_1)
                                  (iadd)
-                                 (invokestatic "Demo" "fact(I)I" 1)
+                                 (invokestatic "Demo" "fact:(I)I" 1)
                                  (imul)
                                  (istore_3))
                                'UNLOCKED
@@ -673,7 +673,7 @@ T
                         (iload_3)
                         (iconst_1)
                         (iadd)
-                        (invokestatic "Demo" "fact(I)I" 1)
+                        (invokestatic "Demo" "fact:(I)I" 1)
                         (imul)
                         (istore_3))
                       'UNLOCKED
