books/projects/symbolic/generic/factorial-jvm-correct.lisp
@@ -92,7 +92,7 @@ method referred to in "Inductive Assertions and Operational Semantics".
         (t
          (let ((n (nth 0 (locals (top-frame (th) s)))))
            (and (equal (program (top-frame (th) s)) (cdddr *fact-def*))
-                (equal (lookup-class-method "fact(I)I" "Demo" (class-table s))
+                (equal (lookup-class-method "fact:(I)I" "Demo" (class-table s))
                        (cons "Demo" *fact-def*))
                 (equal (sync-flg (top-frame (th) s)) 'UNLOCKED)
                 (intp n0)
@@ -157,7 +157,7 @@ method referred to in "Inductive Assertions and Operational Semantics".
                (cdddr *fact-def*))
         (equal (status (th) s) 'scheduled)
         (equal (sync-flg (top-frame (th) s)) 'unlocked)
-        (equal (lookup-class-method "fact(I)I" "Demo" (class-table s))
+        (equal (lookup-class-method "fact:(I)I" "Demo" (class-table s))
                (cons "Demo" *fact-def*))
         (equal (sdepth (call-stack (th) s)) d0)))
 
